thy/OpenFlow/OpenFlowSerialize.thy
@@ -1,6 +1,8 @@
 theory OpenFlowSerialize
-imports OpenFlowMatches OpenFlowAction Semantics_OpenFlow
+imports OpenFlowMatches OpenFlowAction Semantics_OpenFlow "../Primitive_Matchers/Common_Primitive_toString"
 begin
+
+definition "serialization_test_entry \<equiv> OFEntry 7 {IPv4Dst (PrefixMatch 0xA000201 32), IngressPort ''s1-lan'', L4Dst 0x50 0, L4Src 0x400 0x3FF, IPv4Proto 6, EtherType 0x800} [ModifyField_l2dst 0xA641F185E862, Forward ''s1-wan'']"
 
 (*immitation of http://stackoverflow.com/questions/23864965/string-of-nat-in-isabelle*)
 definition "string_of_word_single lc w \<equiv> (if w < 10 then [char_of_nat (48 + unat w)] else if w < 36 then [char_of_nat ((if lc then 87 else 55) + unat w)] else undefined)"
@@ -21,7 +23,7 @@ termination string_of_word
 	apply(rule div_less_dividend_word)
 	apply(metis WordLemmaBucket.power_not_zero linorder_neqE_nat numeral_less_iff power_zero_numeral semiring_norm(76) word_neq_0_conv)
 	apply(clarsimp)
-	apply(thin_tac _)
+	apply(thin_tac "n \<noteq> 0")
 	apply(metis Suc_1 inc_induct le_def less_eq_Suc_le lt1_neq0 not_degenerate_imp_2_neq_0 power_one power_overflow_simp word_le_less_eq) (* words are fun *)
 done 
 
@@ -43,6 +45,30 @@ definition "serialize_action pids a \<equiv> (case a of
 
 definition "serialize_actions pids \<equiv> intersperse (CHR '','') \<circ> map (serialize_action pids)"
 
-value "serialize_actions (\<lambda>oif. ''42'') [ModifyField_l2dst 0xA641F185E862, Forward ''test'']"
+value "serialize_actions (\<lambda>oif. ''42'') (ofe_action serialization_test_entry)"
+
+definition "prefix_to_string pfx \<equiv> ipv4_cidr_toString (pfxm_prefix pfx, pfxm_length pfx)"
+
+primrec serialize_of_match where
+"serialize_of_match pids (IngressPort p) = ''in_port='' @ pids p" |
+"serialize_of_match _ (VlanId i) = ''dl_vlan='' @ string_of_word True 10 i" |
+"serialize_of_match _ (VlanPriority _) = undefined" | (* uh, äh\<dots> We don't use that anyway\<dots> *)
+"serialize_of_match _ (EtherType i) = ''dl_type=0x'' @ string_of_word True 16 i" |
+"serialize_of_match _ (EtherSrc m) = ''dl_src='' @ serialize_mac m" |
+"serialize_of_match _ (EtherDst m) = ''dl_dst'' @ serialize_mac m" |
+"serialize_of_match _ (IPv4Proto i) = ''nw_proto='' @ string_of_word True 10 i" |
+"serialize_of_match _ (IPv4Src p) = ''nw_src='' @ prefix_to_string p" |
+"serialize_of_match _ (IPv4Dst p) = ''nw_dst='' @ prefix_to_string p" |
+"serialize_of_match _ (L4Src i m) = ''tp_src='' @ string_of_word True 10 i @ (if m = max_word then [] else ''/'' @ string_of_word True 16 m)" |
+"serialize_of_match _ (L4Dst i m) = ''tp_dst='' @ string_of_word True 10 i @ (if m = max_word then [] else ''/'' @ string_of_word True 16 m)"
+
+definition "serialize_of_matches pids \<equiv> op @ ''hard_timeout=0,idle_timeout=0,'' \<circ> intersperse (CHR '','') \<circ> map (serialize_of_match pids) \<circ> sorted_list_of_set" 
+
+value "serialize_of_matches (\<lambda>oif. ''42'') (ofe_fields serialization_test_entry)"
+
+definition "serialize_of_entry pids e \<equiv> (case e of (OFEntry p f a) \<Rightarrow> ''priority='' @ string_of_word True 10 p @ '','' @ serialize_of_matches pids f @ '','' @ ''action='' @ serialize_actions pids a)"
+
+value "serialize_of_entry (the \<circ> map_of [(''s1-lan'',''42''),(''s1-wan'',''1337'')]) serialization_test_entry"
+
 
 end
